src/Bedrock/End2End/X25519/MontgomeryLadder.v
@@ -1,6 +1,8 @@
 Require Import Coq.Strings.String.
 Require Import Coq.Lists.List.
 Require Import Coq.ZArith.ZArith.
+Require Import Crypto.Util.Decidable.
+Require Import Crypto.Spec.MontgomeryCurve.
 Require Import Crypto.Spec.Curve25519.
 Require Import bedrock2.Map.Separation.
 Require Import bedrock2.Syntax.
@@ -53,25 +55,29 @@ Require Import coqutil.Map.OfListWord Coq.Init.Byte coqutil.Byte.
 Import ProgramLogic.Coercions.
 Local Notation "m =* P" := ((P%sep) m) (at level 70, only parsing) (* experiment*).
 Local Notation "xs $@ a" := (Array.array ptsto (word.of_Z 1) a xs) (at level 10, format "xs $@ a").
-Definition x25519_gallina K U : F (2^255-19) := 
-  @XZ.M.montladder _ F.zero F.one F.add F.sub F.mul F.inv (F.div (F.of_Z _ 486662 - F.of_Z _ 2) (F.of_Z _ 4))
-  (Z.to_nat (Z.log2 (Z.pos order))) (Z.testbit K) U.
+
 Global Instance spec_of_x25519 : spec_of "x25519" :=
-  fnspec! "x25519" out sk pk / (o s p : list Byte.byte) (R : _ -> Prop),
+  fnspec! "x25519" out sk pk / (o s p : list Byte.byte) P (R : _ -> Prop),
   { requires t m := m =* s$@sk * p$@pk * o$@out * R /\
-      length s = 32%nat /\ length p = 32%nat /\ length o = 32%nat /\ byte.unsigned (nth 31 p x00) <= 0x7f;
+      length s = 32%nat /\ length p = 32%nat /\ length o = 32%nat /\
+      byte.unsigned (nth 31 p x00) <= 0x7f /\ Field.feval_bytes(field_parameters:=field_parameters) p = Curve25519.M.X0 P;
     ensures t' m := t=t' /\ m=* s$@sk ⋆ p$@pk ⋆ R ⋆
-      (le_split 32 (x25519_gallina (le_combine s) (Field.feval_bytes p)))$@out }.
+      (le_split 32 (M.X0 (Curve25519.M.scalarmult (le_combine s mod 2^255) P))$@out) }.
 
 Local Instance spec_of_fe25519_from_word : spec_of "fe25519_from_word" := Field.spec_of_from_word.
 Local Instance spec_of_fe25519_from_bytes : spec_of "fe25519_from_bytes" := Field.spec_of_from_bytes.
 Local Instance spec_of_fe25519_to_bytes : spec_of "fe25519_to_bytes" := Field.spec_of_to_bytes.
-Local Instance spec_of_montladder : spec_of "montladder" := spec_of_montladder(Z.to_nat (Z.log2 Curve25519.order)).
+Local Instance spec_of_montladder : spec_of "montladder" :=
+  spec_of_montladder
+    (Z.to_nat (Z.log2 Curve25519.order))
+    Crypto.Spec.Curve25519.field
+    Curve25519.M.a Curve25519.M.b Curve25519.M.b_nonzero (char_ge_3:=Curve25519.char_ge_3).
 
 Local Arguments word.rep : simpl never.
 Local Arguments word.wrap : simpl never.
 Local Arguments word.unsigned : simpl never.
 Local Arguments word.of_Z : simpl never.
+
 Lemma x25519_ok : program_logic_goal_for_function! x25519.
 Proof.
   repeat straightline.
@@ -94,10 +100,10 @@ Proof.
     eapply byte.unsigned_range. }
   repeat straightline.
 
-  seprewrite_in (@Bignum.Bignum_of_bytes _ _ _ _ _ _ 10 a2) H15. { transitivity 40%nat; trivial. }
+  seprewrite_in (@Bignum.Bignum_of_bytes _ _ _ _ _ _ 10 a2) H16. { transitivity 40%nat; trivial. }
 
   straightline_call; ssplit.
-  3: { unfold FElem, Field.FElem in *; extract_ex1_and_emp_in_goal; ssplit.
+  { unfold FElem, Field.FElem in *; extract_ex1_and_emp_in_goal; ssplit.
        { use_sep_assumption. cancel; repeat ecancel_step.
        cancel_seps_at_indices 0%nat 0%nat; trivial. cbn; reflexivity. }
     all : eauto.
@@ -106,7 +112,7 @@ Proof.
   { rewrite H3. vm_compute. inversion 1. }
   repeat straightline.
 
-  cbv [FElem] in H22. extract_ex1_and_emp_in H22.
+  specialize (H23 P ltac:(assumption)). cbv [FElem] in H23. extract_ex1_and_emp_in H23.
   straightline_call; ssplit.
   { ecancel_assumption. }
   { transitivity 32%nat; auto. }
@@ -116,21 +122,20 @@ Proof.
   repeat straightline.
 
   cbv [Field.FElem] in *.
-  seprewrite_in @Bignum.Bignum_to_bytes H25.
-  seprewrite_in @Bignum.Bignum_to_bytes H25.
-  extract_ex1_and_emp_in H25.
+  seprewrite_in @Bignum.Bignum_to_bytes H26.
+  seprewrite_in @Bignum.Bignum_to_bytes H26.
+  extract_ex1_and_emp_in H26.
 
   repeat straightline; intuition eauto.
-  rewrite H29 in *. cbv [x25519_gallina].
-  use_sep_assumption; cancel. eapply RelationClasses.reflexivity.
+  rewrite H30 in *.
+  use_sep_assumption; cancel. reflexivity.
 Qed.
 
 Global Instance spec_of_x25519_base : spec_of "x25519_base" :=
   fnspec! "x25519_base" out sk / (o s : list Byte.byte) (R : _ -> Prop),
-  { requires t m := m =* s$@sk * o$@out * R /\
-      length s = 32%nat /\ length o = 32%nat;
+  { requires t m := m =* s$@sk * o$@out * R /\ length s = 32%nat /\ length o = 32%nat;
     ensures t' m := t=t' /\ m=* s$@sk ⋆ R ⋆
-      (le_split 32 (x25519_gallina (le_combine s) (F.of_Z _ 9)))$@out }.
+      le_split 32 (M.X0 (Curve25519.M.scalarmult (le_combine s mod 2^255) Curve25519.M.B))$@out }.
 
 Lemma x25519_base_ok : program_logic_goal_for_function! x25519_base.
 Proof.
@@ -143,7 +148,7 @@ Proof.
   seprewrite_in (@Bignum.Bignum_of_bytes _ _ _ _ _ _ 10 a2) H13. { transitivity 40%nat; trivial. }
 
   straightline_call; ssplit.
-  3: { unfold FElem, Field.FElem in *; extract_ex1_and_emp_in_goal; ssplit.
+  { unfold FElem, Field.FElem in *; extract_ex1_and_emp_in_goal; ssplit.
        { use_sep_assumption. cancel; repeat ecancel_step.
        cancel_seps_at_indices 0%nat 0%nat; trivial. cbn; reflexivity. }
     all : eauto.
@@ -152,6 +157,7 @@ Proof.
   { rewrite H3. vm_compute. inversion 1. }
   repeat straightline.
 
+  specialize (H20 Curve25519.M.B eq_refl).
   unfold FElem in H20. extract_ex1_and_emp_in H20.
   straightline_call; ssplit.
   { ecancel_assumption. }
@@ -167,8 +173,8 @@ Proof.
   extract_ex1_and_emp_in H23.
 
   repeat straightline; intuition eauto.
-  rewrite H27 in *. cbv [x25519_gallina].
-  use_sep_assumption; cancel. eapply RelationClasses.reflexivity.
+  rewrite H27 in *.
+  use_sep_assumption; cancel. reflexivity.
 Qed.
 
 Require Import coqutil.Word.Naive.
@@ -196,36 +202,38 @@ Definition funcs :=
 Require Import bedrock2.ToCString.
 Definition montladder_c_module := list_byte_of_string (ToCString.c_module funcs).
 
-#[export]
-Instance BWM_RV32IM : FlatToRiscvCommon.bitwidth_iset 32 Decode.RV32IM := eq_refl.
-
-Derive montladder_compiler_result SuchThat
-       (compile
-         (compile_ext_call (funname_env:=SortedListString.map))
-         funcs = Success montladder_compiler_result)
-       As montladder_compiler_result_ok.
+Lemma link_montladder : spec_of_montladder (map.of_list funcs).
 Proof.
-  match goal with x := _ |- _ => cbv delta [x]; clear x end.
-  match goal with |- ?a = _ => set a end.
-  vm_compute.
-  match goal with |- @Success ?A ?x = Success ?e => is_evar e;
-    exact (@eq_refl (result A) (@Success A x)) end.
+  unfold spec_of_montladder, ScalarMult.MontgomeryLadder.spec_of_montladder.
+  unfold funcs.
+  (* use montladder correctness proof *)
+  rewrite montladder_defn.
+  eapply @montladder_correct; try (typeclasses eauto).
+  { reflexivity. }
+  { Decidable.vm_decide. }
+  { Decidable.vm_decide. }
+  { Decidable.vm_decide. }
+  { eapply M.a2m4_nonsq. }
+  { exact I. }
+  { reflexivity. }
+  { eapply CSwap.cswap_body_correct; [|exact I|reflexivity].
+    unfold field_representation, Signature.field_representation, Representation.frep; cbn; unfold n; cbv; trivial. }
+  { eapply fe25519_copy_correct. reflexivity. }
+  { eapply fe25519_from_word_correct. reflexivity. }
+  {
+    cbv [LadderStep.spec_of_ladderstep]; intros.
+    rewrite ladderstep_defn.
+    eapply @LadderStep.ladderstep_correct; try (typeclasses eauto).
+    { cbv [Core.__rupicola_program_marker]; tauto. }
+    { reflexivity. }
+    { apply fe25519_mul_correct. reflexivity. }
+    { apply fe25519_add_correct. reflexivity. }
+    { apply fe25519_sub_correct. reflexivity. }
+    { apply fe25519_square_correct. reflexivity. }
+    { apply fe25519_scmula24_correct. reflexivity. }
+    { ecancel_assumption. } }
+  { unshelve eapply AdditionChains.fe25519_inv_correct_exp; [exact I|reflexivity| | ].
+    { apply fe25519_square_correct. reflexivity. }
+    { apply fe25519_mul_correct. reflexivity. } }
+  { apply fe25519_mul_correct. reflexivity. }
 Qed.
-
-Definition montladder_stack_size := snd montladder_compiler_result.
-Definition montladder_finfo := snd (fst montladder_compiler_result).
-Definition montladder_insns := fst (fst montladder_compiler_result).
-Definition montladder_bytes := Pipeline.instrencode montladder_insns.
-Definition montladder_symbols : list byte := Symbols.symbols montladder_finfo.
-
-
-Require riscv.Utility.InstructionNotations.
-Require riscv.Utility.InstructionCoercions.
-Module PrintAssembly.
-  Import riscv.Utility.InstructionNotations.
-  Import riscv.Utility.InstructionCoercions.
-  Unset Printing Coercions.
-
-  (* Compute garagedoor_finfo. (* fe25519_mul is more than 10KB in just one function *) *)
-  Goal True. let r := eval cbv in montladder_insns in idtac (* r *). Abort.
-End PrintAssembly.
